\documentclass[12pt]{article}
 \usepackage[margin=1in]{geometry} 
\usepackage{amsmath,amsthm,amssymb,amsfonts}
 
\newcommand{\N}{\mathbb{N}}
\newcommand{\Z}{\mathbb{Z}}
\newcommand{\boner}{\delta_{M}^{*}}
 
\newenvironment{problem}[2][Problem]{\begin{trivlist}
\item[\hskip \labelsep {\bfseries #1}\hskip \labelsep {\bfseries #2.}]}{\end{trivlist}}
 
\begin{document}
\title{HW 3}
\author{Dana Nikolaeva Chambourova}
\maketitle
 
\begin{problem}{1}
homomorphism $h:\epsilon \implies \Delta^*$\\
%% format the piece wise function
if $h(w) = \{ \epsilon$ \text{, if} $ w = \epsilon $\\
$ h(a)h(\mu) $ \text{, if } $w=an$ \text{ where } $a \in \Sigma $ \text{ , } $\mu \in \Sigma^* \}$\\
$h^*(L) = \{ h(w) | w \in L \}$ \text{ where } $L \subseteq \Sigma^*$\\
$h^{-1} = \{ h(w) | h(w) \in L \}$ \\ \\ 
$\Sigma =  \{ a,b \}$\text{,  } $h(a) = 01$\\ 
$\Delta = \{0,1\}$\text{,  } $h(b) = 10$\\ \\
% format part a and part b
\textbf{a)}\\
$h^{-1}( \{0101\} )= (ab)$\\
$h^{-1}( \{00\} )= \emptyset$\\
$h^{-1}( \{001\} )= \emptyset$\\
$h^{-1}( \{1001\} )= (ba)$ \\ \\
\textbf{b)}\\
$L = L((00 + 1)^*)$\\
$h^{-1}(L) = (ba)^*$\\
$h(h^{-1}(L))=h((ba)^*) = (1001)^*$
\end{problem}

\begin{problem}{2}\text{Regular language are closed under inverse homomorphic images}\\
if $h:\Sigma \implies \Delta^*$ and $L \subseteq \Delta^*$ is regular than $h^{-1} $ is regular\\ 
\textbf{a)}
$w \in \Sigma^*$ , $ d_{n}^*(s^{'}w) = \delta_{M}^{*}(s, h(w)) $\\ 
\\ \textbf{b)} Prove the correctness statement by induction on the length w	\\
\begin{proof}
We will do induction on $|w|$\\ 
\underline{Base Case}: \\
When $|w|$, $ w=\epsilon $\\
$\boner(s^{'},w) = \boner(\delta, h(w))$\\
$\boner(s^{'},w) = \boner(\delta, h(\epsilon)) $\\ \linebreak
Since $s'^{*} = s$\\
$\boner (s,\epsilon)= \boner(s,h(\epsilon)) $\\ \linebreak
By definition of a homomorphism\\ 
$h(\epsilon) = \epsilon$\\
$\boner(s,\epsilon) = \boner(s,\epsilon)$ \\ \\
\underline{Inductive Hypothesis}: $\forall w $ \text{where} $ |w| < n$ , $\boner(s,w) = \boner(s',h(w))$ 
\\ \underline{Induction Step}:\\
Let w be a string such that $|w|=\mu$\\
And as we know $s=s'$ then \\
$\boner(s,w) = \boner(s,h(w))=$\\
Let $w=an$, $a \in \Sigma $, $\mu \in \Sigma^*$\\
$\boner(s,a*m) = \boner(s, h(a)*h(\mu))$\\
$\boner(\delta(s,a),\mu) = \boner(\boner(s,h(a), h(\mu))$\\
$\boner(\delta(s,a),\mu) = \boner(\boner(s,a),\mu)$

\end{proof}
\end{problem}
\end{document}
